\PassOptionsToPackage{table}{xcolor}
\documentclass[9pt,xcolor=x11names,compress]{beamer}

%% General document %%%%%%%%%%%%%%%%%%%%%%%%%%%%%%%%%%
\usepackage{graphicx}
\usepackage{tikz}
\usetikzlibrary{decorations.fractals,lindenmayersystems}
%%%%%%%%%%%%%%%%%%%%%%%%%%%%%%%%%%%%%%%%%%%%%%%%%%%%%%


%% Beamer Layout %%%%%%%%%%%%%%%%%%%%%%%%%%%%%%%%%%
\useoutertheme[subsection=false,shadow]{miniframes}
\useinnertheme{default}
\usefonttheme{serif}
\usepackage{palatino}

\setbeamerfont{title like}{shape=\scshape}
\setbeamerfont{frametitle}{shape=\scshape}

\setbeamercolor*{lower separation line head}{bg=DeepSkyBlue4} 
\setbeamercolor*{normal text}{fg=black,bg=white} 
\setbeamercolor*{alerted text}{fg=DeepSkyBlue4} 
\setbeamercolor*{example text}{fg=black} 
\setbeamercolor*{structure}{fg=black} 
 
\setbeamercolor*{palette tertiary}{fg=black,bg=black!10} 
\setbeamercolor*{palette quaternary}{fg=black,bg=black!10} 

\setbeamertemplate{blocks}[rounded][shadow=true]
\setbeamercolor{block title}{bg=DeepSkyBlue4}
\setbeamercolor{block title example}{bg=DeepSkyBlue4}
\setbeamercolor{block body}{bg=black!15!white}
\setbeamercolor{block body example}{bg=black!15!white}

\setbeamertemplate{navigation symbols}{}
%%%%%%%%%%%%%%%%%%%%%%%%%%%%%%%%%%%%%%%%%%%%%%%%%%

\title{Lesson 11: Rules of Differentiation---Product and Quotient Rules}
\author[Francisco Blanco-Silva]{Francisco Blanco-Silva}
\institute[USC]{University of South Carolina}
\date{
\pgfdeclarelindenmayersystem{Gosper curve}{
	\rule{XF -> XF+YF++YF-XF--XFXF-YF+}
	\rule{YF -> -XF+YFYF++YF+XF--XF-YF}
}
\begin{tikzpicture}[color=DeepSkyBlue4]
\draw [l-system={Gosper curve, axiom=XF, order=5, step=0.6pt, angle=60}]
lindenmayer system; 
\end{tikzpicture}
}

\begin{document}
\frame{\titlepage}

\section{What do we know?}
\subsection{}

\begin{frame}
\frametitle{What do we know?}
\framesubtitle{The General Program}
\begin{columns}[T]
\begin{column}{0.6\linewidth}
\begin{itemize}
\item Functions
\begin{itemize}
\item $x-$ and $y-$\alert{intercepts} ($f(x)=0$, $f(0)$)
\item \alert{Change} from $x=a$ to $x=b$ 
\begin{equation*}
	\Delta y = f(b)-f(a)
\end{equation*}
\item \alert{Average Rate of Change} from $x=a$ to $x=b$
\begin{equation*}
ARC=\frac{\Delta y}{\Delta x}=\frac{f(b)-f(a)}{b-a} 
\end{equation*}
\item \alert{Relative Change} from $x=a$ to $x=b$
\begin{equation*}
RC=\frac{\Delta y}{f(a)}=\frac{f(b)-f(a)}{f(a)}
\end{equation*}
\item \alert{Instantaneous Rate of Change} at $x=a$
\begin{equation*}
	f'(a)
\end{equation*}
\end{itemize}
\end{itemize}
\end{column}
\begin{column}{0.4\linewidth}
\begin{itemize}
	\item Linear Functions: $f(x)=b+mx$
	\item Exponential Functions $P_0 a^t = P_0 (1+r)^t = P_0 e^{kt}$
	\item Power Functions \newline \makebox[1cm]{} $kx^p$
	\item Polynomials $a_0+a_1x+a_2x^2+\dotsb+a_n x^n$
\end{itemize}
\end{column}
\end{columns}
\end{frame}

\begin{frame}\frametitle{What do we know?}
\framesubtitle{Rules of Differentiation}
\begin{description}
	\item[\textbf{D1}] $f(x)=c,\quad \alert{f'(x)=0}$
	\item[\textbf{D2}] $f(x)=x,\quad \alert{f'(x)=1}$
	\item[\textbf{D3}] $h(x)=f(x)+g(x),\quad \alert{h'(x)=f'(x)+g'(x)}$
	\item[\textbf{D4}] $h(x)=f(x)-g(x),\quad \alert{h'(x)=f'(x)-g'(x)}$
	\item[\textbf{D5}] $h(x)=c\cdot f(x),\quad \alert{h'(x)=c\cdot f'(x)}$
	\item[\textbf{\alert{D6}}] $f(x)=x^n,\quad \alert{f'(x)=nx^{n-1}}$
	\item[\textbf{\alert{D7}}] $f(x)=e^x,\quad \alert{f'(x)=e^x}$
	\item[\textbf{\alert{D8}}] $f(x)=a^x,\quad \alert{f'(x)=a^x \ln a}$
	\item[\textbf{\alert{D9}}] $f(x)=\ln x,\quad \alert{f'(x)=\tfrac{1}{x}}$
	\item[\textbf{D10}] 
	\begin{itemize}
		\item $f(x)=g(x)^n,\quad \alert{f'(x)=ng(x)^{n-1}g'(x)}$
		\item $f(x)=e^{g(x)},\quad \alert{f'(x)=g'(x)e^{g(x)}}$
		\item $f(x)=a^{g(x)},\quad \alert{f'(x)=g'(x)\ln a\,a^{g(x)}}$
		\item $f(x)=\ln g(x),\quad \alert{f'(x)=\frac{g'(x)}{g(x)}}$
	\end{itemize}
\end{description}
\end{frame}

\section{The Product and Quotient Rule}
\subsection{Rules}
\begin{frame}\frametitle{The Product and Quotient Rules}
\framesubtitle{Two more rules}
\begin{description}
\item[\textbf{D11}] \alert{The Product Rule}

If $h(x)=f(x)\cdot g(x)$, then $h'(x)=f'(x)\cdot g(x) + f(x)\cdot g'(x)$.
\item[\textbf{D12}] \alert{The Quotient Rule} 

If $h(x)=\dfrac{f(x)}{g(x)}$, then $h'(x)=\dfrac{f'(x)\cdot g(x) - f(x)\cdot g'(x)}{g(x)^2}$.
\end{description}
\pause You may have seen these two rules with the $u,v$ notation:
\begin{description}
	\item[\textbf{D11}] $\big( u\cdot v \big)' = u' v + u v'$.
	\item[\textbf{D12}] $\Big( \dfrac{u}{v} \Big)' = \dfrac{u'v-uv'}{v^2}$.
\end{description}
\pause No matter what technique you use, make sure you get the order of the parts and the sign right.
\end{frame}

\subsection{Examples}

\begin{frame}\frametitle{The Product and Quotient Rule}
\framesubtitle{Examples}
\begin{block}
	{Find the derivative of the following functions}
	\begin{itemize}
		\item $f(x)=\only<1>{(x^2-4)(4x^6-7x+2)}\only<2->{\underbrace{(x^2-4)}_{u} \underbrace{(4x^6-7x+2)}_{v}}$
		\begin{align*}
			\uncover<3->{u&=x^2-4} \uncover<4->{&u'&=2x} \\
			\uncover<3->{v&=4x^6-7x+2} \uncover<4->{&v'&=24x^5-7} 
		\end{align*}
		\begin{equation*}
			\alert{\uncover<5->{f'(x)=u'v+uv'}\uncover<6->{= 2x(4x^6-7x+2)+(x^2-4)(24x^5-7)}}
		\end{equation*}
		\item $f(x)=\only<1-6>{\big(x+\sqrt[3]{x}\big)(5x^2+e^x)}\only<7->{\underbrace{(x+x^{1/3})}_{u}\underbrace{(5x^2+e^x)}_{v}}$
		\begin{align*}
			\uncover<8->{u&=x+x^{1/3}} \uncover<9->{&u'&=1+\tfrac{1}{3}x^{-2/3}} \\
			\uncover<8->{v&=5x^2+e^x} \uncover<9->{&v'&=10x+e^x}
		\end{align*}
		\begin{equation*}
			\alert{\uncover<9->{f'(x)=u'v+uv'}\uncover<10->{=(1+\tfrac{1}{3}x^{-2/3})(5x^2+e^x)+(x+x^{1/3})(10x+e^x)}}
		\end{equation*}
	\end{itemize}
\end{block}
\end{frame}

\begin{frame}\frametitle{The Product and Quotient Rule}
\framesubtitle{Examples}
\begin{block}
	{Find the derivative of the following functions}
	\begin{itemize}
		\item $f(x)=\only<1>{(3x^3-\ln x)\big(x^5-\sqrt{x}\big)}\only<2->{\underbrace{(3x^3-\ln x)}_{u} \underbrace{\big(x^5-x^{1/2}\big)}_{v}}$
		\begin{align*}
			\uncover<3->{u&=3x^3-\ln x} \uncover<4->{&u'&=9x^2-\tfrac{1}{x}} \\
			\uncover<3->{v&=x^5-x^{1/2}} \uncover<4->{&v'&=5x^4-\tfrac{1}{2}x^{-1/2}} 
		\end{align*}
		\begin{equation*}
			\alert{\uncover<5->{f'(x)=u'v+uv'}\uncover<6->{= \big(9x^2-\tfrac{1}{x}\big)\big(x^5-x^{1/2}\big)+(3x^3-\ln x)\big(5x^4-\tfrac{1}{2}x^{-1/2}\big)}}
		\end{equation*}
		\item $f(x)=\only<1-6>{\big(x^3+\sqrt{x}\big)(5x^2+e^x)}\only<7->{\underbrace{(x^3+x^{1/2})}_{u}\underbrace{(5x^2+e^x)}_{v}}$
		\begin{align*}
			\uncover<8->{u&=x^3+x^{1/2}} \uncover<9->{&u'&=3x^2+\tfrac{1}{2}x^{-1/2}} \\
			\uncover<8->{v&=5x^2+e^x} \uncover<9->{&v'&=10x+e^x}
		\end{align*}
		\begin{equation*}
			\alert{\uncover<9->{f'(x)=u'v+uv'}\uncover<10->{=(3x^2+\tfrac{1}{2}x^{-1/2})(5x^2+e^x)+(x^3+x^{1/2})(10x+e^x)}}
		\end{equation*}
	\end{itemize}
\end{block}
\end{frame}

\begin{frame}\frametitle{The Product and Quotient Rule}
\framesubtitle{Examples}
\begin{block}
	{Find the derivative of the following function}
	\begin{equation*}
		f(x)=\dfrac{3x^2+\ln x}{1-3x^{4/3}+2^x}\alert{\only<2->{\quad\displaystyle{\genfrac{}{}{0pt}{}{\longleftarrow u}{\longleftarrow v}}}}
	\end{equation*}
\end{block}
		\begin{align*}
			\uncover<2->{u&=3x^2+\ln x} \uncover<3->{&u'&=6x+\tfrac{1}{x}} \\
			\uncover<2->{v&=1-3x^{4/3}+2^x} \uncover<3->{&v'&=-4x^{1/3}+2^x\ln 2} 
		\end{align*}
		\begin{align*}
			\uncover<4->{\alert{f'(x)}&\alert{=\frac{u'v-uv'}{v^2}}}\\
			\uncover<5->{&\alert{=\frac{\big(6x+\tfrac{1}{x}\big)(1-3x^{4/3}+2^x)-(3x^2+\ln x)(-4x^{1/3}+2^x\ln 2)}{(1-3x^{4/3}+2^x)^2}}}
		\end{align*}
\end{frame}

\begin{frame}\frametitle{The Product and Quotient Rule}
\framesubtitle{Examples}
\begin{block}
	{Find the derivative of the following function}
	\begin{equation*}
		f(x)=\dfrac{\pi + 2\pi x - \ln \pi + \pi^x}{e-e^x+3x^2}\alert{\only<2->{\quad\displaystyle{\genfrac{}{}{0pt}{}{\longleftarrow u}{\longleftarrow v}}}}
	\end{equation*}
	\end{block}
		\begin{align*}
			\uncover<2->{u&=\pi+2\pi x-\ln \pi+\pi^x} \uncover<3->{&u'&=2\pi + \pi^x \ln\pi} \\
			\uncover<2->{v&=e-e^x+3x^2} \uncover<3->{&v'&=-e^x+6x}
		\end{align*}
		\begin{align*}
			\uncover<4->{\alert{f'(x)}&\alert{=\frac{u'v-uv'}{v^2}}}\\
			\uncover<5->{&\alert{=\frac{(2\pi+\pi^x \ln\pi)(e-e^x+3x^2)-(\pi+2\pi x-\ln\pi+\pi^x)(-e^x+6x)}{(e-e^x+3x^2)^2}}}
		\end{align*}
\end{frame}

\begin{frame}\frametitle{The Product and Quotient Rule}
\framesubtitle{Examples}
\begin{block}
	{Find the derivative of the following function}
	\begin{equation*}
		f(x)=\only<1>{\big(e^{x^3}-\ln (4x^6-5)\big)\Big(3 + \frac{1}{\sqrt{3x-9}}\Big)}\only<2->{\underbrace{\big(e^{x^3}-\ln (4x^6-5)\big)}_{u}\underbrace{\Big(3 + \frac{1}{\sqrt{3x-9}}\Big)}_{v}}
	\end{equation*}
\end{block}
\begin{align*}
	\uncover<2->{u&=e^{x^3}-\ln(4x^6-5)} \uncover<3->{&u'&=3x^2 e^{x^3} - \dfrac{24x^5}{4x^6-5}} \\
	\uncover<2->{v&=3+(3x-9)^{-1/2}} \uncover<4->{&v'&=-\tfrac{3}{2}(3x-9)^{-3/2}}
\end{align*}
\begin{align*}
	\uncover<5->{\alert{f'(x)}&\alert{=u'v+uv'}\\}
	\uncover<6->{&\alert{=\Big(3x^2 e^{x^3} - \frac{24x^5}{4x^6-5} \Big)\big(3+(3x-9)^{-1/2}\big)} \\}
	\uncover<6->{&\quad\alert{+ \big( e^{x^3}-\ln(4x^6-5)\big) \big( -\tfrac{3}{2}(3x-9)^{-3/2}\big)}}
\end{align*}
\end{frame}

\begin{frame}\frametitle{The Product and Quotient Rule}
\framesubtitle{Examples}
\begin{block}
	{Find the derivative of the following function}
	\begin{equation*}
	f(x)=\frac{\big(5x^7-4x+3\sqrt{x}\big)^2}{\ln\big(3-4x^{2/3}\big)} \alert{\uncover<2->{\quad \displaystyle{\genfrac{}{}{0pt}{}{\longleftarrow u}{\longleftarrow v}}}}
	\end{equation*}
\end{block}
\begin{align*}
	\uncover<2->{u&=\big(5x^7-4x+3x^{1/2}\big)^2} \uncover<3->{&u'&=2\big(5x^7-4x+3x^{1/2}\big)\big(35x^6-4+\tfrac{3}{2}x^{-1/2}\big)} \\
	\uncover<2->{v&=\ln \big( 3-4x^{2/3}\big)} \uncover<4->{&v'&=\frac{-\tfrac{8}{3}x^{-1/3}}{3-4x^{2/3}}}
\end{align*}
\begin{align*}
	\uncover<5->{\alert{f'(x)}&\alert{=\frac{u'v-uv'}{v^2}}} 
	\uncover<6->{\alert{=\text{ain't nobody got time for that!}}}
\end{align*}
\end{frame}

\end{document}